autoclrs/common/CLRS.Common.Complexity.Sorting.Class.fst
@@ -1,0 +1,55 @@
+module CLRS.Common.Complexity.Sorting.Class
+open Pulse
+#lang-pulse
+module A = Pulse.Lib.Array
+module SZ = FStar.SizeT
+module Seq = FStar.Seq
+module TC = FStar.Tactics.Typeclasses
+module TO = Pulse.Lib.TotalOrder
+module MR = Pulse.Lib.MonotonicGhostRef
+open FStar.Order
+
+let rec count (#t:Type) (x:t) (s:Seq.seq t)
+: GTot nat (decreases Seq.length s)
+= if Seq.length s = 0 then 0
+  else if Seq.head s == x
+  then 1 + count x (Seq.tail s)
+  else count x (Seq.tail s)
+
+let permutation 
+      (#t:Type)
+      (s0 s1:Seq.seq t)
+= forall (x:t). count x s0 == count x s1
+    
+let sorted 
+      (#t:Type)
+      {| TO.total_order t |}
+      (s:Seq.seq t)
+= let open TO in
+  forall (i j:nat).{:pattern (Seq.index s i); (Seq.index s j)}
+  i <= j /\ j < Seq.length s ==> Seq.index s i <=? Seq.index s j
+
+let preorder_nat : FStar.Preorder.preorder nat = (fun (x y:nat) -> b2t (x <= y))
+
+let ticks_t = MR.mref #nat preorder_nat
+
+let instrumented_total_order (a:Type) (ord:Pulse.Lib.TotalOrder.total_order a) (ctr:ticks_t) =
+  fn (x y:a) (#i:erased nat)
+  requires MR.pts_to ctr #1.0R i
+  returns o:order
+  ensures MR.pts_to ctr #1.0R (i + 1)
+  ensures pure (o == x `ord.TO.compare` y)
+
+class array_sort (a:Type) (f: nat -> nat) = {
+  sort: (fn (arr:A.array a)
+            (len:SZ.t) 
+            (ctr:ticks_t)
+            (#ord:erased (TO.total_order a))
+            (iord:instrumented_total_order a ord ctr)
+            (#s:erased (Seq.seq a)) (#i:erased nat)
+         requires arr |-> s ** pure (A.length arr == SZ.v len) ** MR.pts_to ctr #1.0R i
+         ensures exists* s' ticks. 
+           arr |-> s' **
+           MR.pts_to ctr #1.0R ticks **
+           pure (sorted #_ #ord s' /\ permutation s s' /\ ticks <= i + f (Seq.length s)))
+}
